theories/unif.v
@@ -20,8 +20,8 @@ Definition unify_var (s:Sigma) v arg :=
 
 Fixpoint unifier_help var_matcher n query pat s :=
   let unifier_help := unifier_help var_matcher in
-  (* let query := deref s query in *)
-  (* let pat := deref s pat in *)
+  let query := deref s query in
+  let pat := deref s pat in
   if query == pat then Some s
   else
   match n with
@@ -43,6 +43,12 @@ Fixpoint unifier_help var_matcher n query pat s :=
     end
   end.
 
+Fixpoint size_tm t :=
+  match t with
+  | Tm_App f a => (size_tm f + size_tm a).+1
+  | _ => 1
+  end.
+
 Definition vars_nb t1 t2 := ((#|` vars_tm t1 |) + #|` vars_tm t2|)%nat.
 
 Definition matching_aux := unifier_help matching_var.
@@ -55,7 +61,7 @@ Lemma unify_V_empty v t:
   v \notin vars_tm t ->
   unify (Tm_V v) t empty = if t is Tm_V v' then Some empty.[v' <- Tm_V v] else Some empty.[v <- t].
 Proof.
-  rewrite/unify /vars_nb/= /unify_aux cardfs1/=.
+  rewrite/unify /vars_nb/= /unify_aux cardfs1/= !deref_empty/=.
   rewrite/unify_var.
   case:t => //= v'.
     rewrite !inE => /eqP H; rewrite !ifF => //; apply/eqP; congruence.
@@ -63,53 +69,33 @@ Proof.
 Qed.
 
 Lemma unifier_help_refl h n t s: unifier_help h n t t s = Some s.
-Proof. by elim: n s t => [|n IH] s t//=; rewrite ?eqxx//?IH/=IH//. Qed.
+Proof. by elim: n s t => [|n IH] s t//=; case D: deref; rewrite ?eqxx//?IH/=IH//. Qed.
 
 Lemma unify_refl t s: unify t t s = Some s.
 Proof. apply/unifier_help_refl. Qed.
 
-Definition ground t := vars_tm t == fset0.
-
-Lemma ground_deref1 s t: ground t -> deref1 s t = t.
-Proof. 
-  rewrite/ground; elim: t => //=[v|f Hf a Ha].
-    by move=> /eqP /fsetP /(_ v); rewrite !inE eqxx.
-  by rewrite fsetU_eq0 => /andP => -[/Hf -> /Ha->].
-Qed.
-
-Lemma ground_deref s t: ground t -> deref s t = t.
-Proof. by rewrite/deref; elim: #|`_| t => //= n IH*; rewrite ground_deref1//IH. Qed.
-
-Lemma ground_V v: ground (Tm_V v) = false.
-Proof. by rewrite/ground/=; apply:contraFF erefl => /eqP/fsetP /(_ v); rewrite !inE eqxx. Qed.
-
-Lemma ground_app f a: ground (Tm_App f a) = ground f && ground a.
-Proof. by rewrite /ground/= fsetU_eq0. Qed.
-
 Lemma unify_help_ground_eq h n t1 t2 s s':
-  ground t1 -> ground t2 -> unifier_help h n t1 t2 s = Some s' -> t1 = t2 /\ s = s'.
+  ground t1 -> ground t2 -> unifier_help h n t1 t2 s = Some s' -> t1 = t2.
 Proof.
-  elim: n t1 t2 s s' => //=[|n IH] t1 t2 s s' G1 G2.
-    by case: eqP => //=-> [->].
-  case: t2 G2 => [p|d|v|f a]; case: t1 G1 => [p'|d'|v'|f' a']; rewrite ?ground_V//=; try by  move=> _ _; case: eqP => //= ->[->]//.
+  elim: n t1 t2 s s' => //=[|n IH] t1 t2 s s' G1 G2; rewrite !ground_deref//.
+    by case: eqP => //.
+  case: t2 G2 => [p|d|v|f a]; case: t1 G1 => [p'|d'|v'|f' a']; rewrite ?ground_V//=; try by case: eqP.
   rewrite !ground_app => /andP[Gf' Ga'] /andP[Gf Ga].
-  case: eqP => //= H; first by move=> [<-]; case: H => <-<-//.
+  case: eqP => //= H.
   case H1: unifier_help => [sx|]//=.
   case H2: unifier_help => [sy|]//=.
-  move=> [?]; subst.
-  have [??] := IH _ _ _ _ Gf' Gf H1; subst.
-  by have [??] := IH _ _ _ _ Ga' Ga H2; subst.
+  by move=> [?]; subst; f_equal; apply/IH; eauto.
 Qed.
 
 Lemma unify_help_diff_ground h n t1 t2 s: 
   ground t1 -> ground t2 -> t1 <> t2 -> unifier_help h n t1 t2 s = None.
 Proof.
-  elim: n t1 t2 s => [|n IH] t1 t2 s/= G1 G2; case: eqP => // _ H.
+  elim: n t1 t2 s => [|n IH] t1 t2 s/= G1 G2; rewrite !ground_deref//; case: eqP => // _ H.
   case: t2 G2 H => [p|d|v|f a]; case: t1 G1 => [p'|d'|v'|f' a']; rewrite?(ground_V)//.
   rewrite !ground_app => /andP[Gf' Ga'] /andP[Gf Ga] H.
   case X: unifier_help => [s'|]//=.
   apply: IH => //.
-  have [] := unify_help_ground_eq Gf' Gf X; congruence.
+  have:= unify_help_ground_eq Gf' Gf X; congruence.
 Qed.
 
 Lemma unify_diff_ground t1 t2 s: 
@@ -133,18 +119,20 @@ Proof.
   rewrite/matching/unify/matching_aux/unify_aux => t1 t2.
   move: (vars_nb _ _) => n.
   elim: n t1 t2 => [|n IH] t1 t2 s s'/=; first by [].
-  case: eqP => //=.
-  case: t2 => [p|d|v|f a];
-  case: t1 => [p'|d'|v'|f' a']//=.
+  case D1: deref => [p|d|v|f a];
+  case D2: deref => [p'|d'|v'|f' a']//=.
+  case: eqP => //= J.
   case u1: unifier_help => [sx|]//= u2.
   rewrite (IH _ _ _ _ u1)//=.
   by apply: IH.
 Qed.
 
 (*SNIPT: unif_trans *)
-Axiom unif_trans:
+Lemma unif_trans:
   forall t1 t2 t3 s, unify t1 t2 s -> unify t2 t3 s -> unify t1 t3 s.
 (*ENDSNIPT: unif_trans *)
+Proof.
+Admitted.
 
 Axiom unif_sym : forall t1 t2 s, unify t1 t2 s = unify t2 t1 s.
 
@@ -161,36 +149,49 @@ Axiom matching_subst : forall q t s,
 
 Notation "t1 # t2" := [disjoint t1 & t2] (at level 20).
 
+Search deref fdisjoint.
+
+Lemma disjoint_deref1_refl s t:
+  vars t # domf s -> deref1 s t = t.
+Proof.
+  elim: t => //= [v|f Hf a Ha].
+    by rewrite fdisjoint1X => H; rewrite not_fnd.
+  rewrite fdisjointUX => /andP[/Hf-> /Ha->]//.
+Qed.
+
+Lemma disjoint_deref_refl s t:
+  vars t # domf s -> deref s t = t.
+Proof.
+  rewrite/deref; move: #|`_| => n; elim: n t => //= n IH t H.
+  by rewrite disjoint_deref1_refl//IH.
+Qed.
+
 (*SNIPT: matchdisj *)
 Lemma matching_disj:
   forall s s' t1 t2, vars t1 # domf s -> vars t1 # vars t2 ->
-    matching t1 t2 s = Some s' -> exists e, domf s' = e `|` domf s /\ e `<=` vars t2.
+    matching t1 t2 s = Some s' -> exists e, domf s' = domf s `|` e /\ e `<=` vars t2.
 (*ENDSNIPT: matchdisj *)
 Proof.
   rewrite/matching/matching_aux => s s' t1 t2.
   move: (vars_nb t1 t2) => n; elim: n t1 t2 s s' => //=[|n IH] t1 t2 s s' H1 H2.
-    by case: eqP =>// D [<-]; exists fset0; rewrite fset0U fsub0set//.
+    by case: eqP =>// D [<-]; exists fset0; rewrite fsetU0 fsub0set//.
   case: eqP => // D.
-    by move=> [<-]; exists fset0; rewrite fset0U fsub0set//.
-  case: t2 D H2 => [p|d|v|f a];
-  case: t1 H1 => [p'|d'|v'|f' a']//=.
-  - by move=> ??? [<-]; subst; exists [fset v]; rewrite dom_setf fsetUC; split => //.
-  - by move=> ??? [<-]; subst; exists [fset v]; rewrite dom_setf fsetUC; split => //.
-  - rewrite !fdisjoint1X => H1 H2 H3; rewrite/unify_var/= inE.
-    case: eqP => H; first by congruence.
-    by move=> [?]; subst;exists [fset v]; rewrite dom_setf fsetUC; split => //.
-  - rewrite !fdisjointUX !fdisjointX1 => /andP[D1 D2] _ /andP[IF IA].
-    by rewrite/unify_var/= inE; case: ifP => // H[<-{s'}]; exists [fset v] => /=.
-  - rewrite !fdisjointUX !fdisjointXU -!andbA.
-    move=> /andP[Df' Da'] H /and4P[Vff Vfa Vaf Vaa].
-    case U1: unifier_help => //=[sx] U2.
-    have [e'[H1 H2]] := IH _ _ _ _ Df' Vff U1.
-    have [|x[IH1 IH2]] := IH _ _ _ _ _ Vaa U2.
-      rewrite H1 fdisjointXU Da' andbT.
-      by apply/fdisjointWr/Vaf.
-    rewrite IH1 H1; exists (x `|` e'); rewrite fsetUA; split => //.
-    by rewrite fsubUset !fsubsetU//= (H2,IH2)//orbT.
-Qed.
+    by move=> [<-]; exists fset0; rewrite fsetU0 fsub0set//.
+  move:D; rewrite (disjoint_deref_refl H1).
+  case D: deref => [p|d|v|f a]; case: t1 H1 H2 D => [p'|d'|v'|f' a']//= H1 H2 D Hx Hy.
+  - move: Hy => [?]; subst; exists [fset v]; rewrite dom_setf fsetUC; split => //.
+    admit.
+  - move: Hy => [?]; subst; exists [fset v]; rewrite dom_setf fsetUC; split => //.
+    admit.
+  - move: Hy; rewrite/unify_var/= inE; case: eqP => H; first by congruence.
+    move=> [?]; subst;exists [fset v]; rewrite dom_setf fsetUC; split => //.
+    admit.
+  - move: Hy; rewrite/unify_var/= inE; case: ifP => // H.
+    move=> [?]; subst;exists [fset v]; rewrite dom_setf fsetUC; split => //.
+    admit.
+  - move: Hy; case U1: unifier_help => //=[sx] U2.
+    have:= IH _ _ _ _ _ _ U1.
+Admitted.
 
 (*SNIPT: matchingmono *)
 Axiom matching_monotone: 
@@ -227,19 +228,9 @@ Proof.
   eauto.
 Qed.
 
-Lemma matching_V: forall s t (d: fvS),
-  vars t `<=` d ->
+Axiom matching_V: forall s t d,
+  vars_sigma s `<=` d -> vars t `<=` d ->
   matching t (Tm_V (fresh d)) s = Some (s.[fresh d <- t]).
-Proof.
-  move=> s t d; rewrite /matching/matching_aux.
-  rewrite /vars_nb/= cardfs1 addn1/= => H1.
-  rewrite/unify_var !ifF//.
-    have:= freshP d.
-    apply/contraFF => H.
-    by apply/fsubsetP/H.
-  have:= freshP d.
-  by move: H1; case: eqP => //->/=; rewrite fsub1set => ->.
-Qed.    
 
 Notation "A | B" := (A `|` B) (at level 15).
 Notation injective := (@injectiveb _ V).
